update

lean4/Crypto/Structure.lean
@@ -18,6 +18,7 @@ def AddToContext (lctx : LocalContext) (h : Name) (t : Expr) : MetaM (LocalConte
 #check withMainContext
 #check evalGeneralize
 #check Parser.Tactic.generalize
+
 -- #check Parser.Tactic.have
 structure FieldData where
 (fvar : Expr)
@@ -25,69 +26,55 @@ structure FieldData where
 (depends : NameSet)
 (isProp : Bool)
 
-#print String
-#print Format
 open Std.Format
 
 instance : ToFormat NameSet :=
 ⟨λ x => fmt x.toList⟩
 
 instance : ToFormat FieldData :=
-⟨λ ⟨a, b, c, d⟩ => group (nest 1 (fmt "⟨"  ++ fmt a ++ fmt "," ++ line ++ fmt b ++ fmt "," ++ line ++ fmt c ++ fmt "," ++ line ++ fmt d ++ fmt "⟩"))⟩
+⟨λ ⟨a, b, c, d⟩ => group (nest 1 (fmt "⟨"  ++ fmt a ++ fmt "," ++ line ++ fmt b ++ fmt "," ++ line
+++ fmt c ++ fmt "," ++ line ++ fmt d ++ fmt "⟩"))⟩
 
--- /-- Add fields to context, and returns data -/
--- def AddFieldsToContext (lctx : LocalContext) (nm : Name) (pref : Name) (args : Array Expr) :
---   MetaM (LocalContext × Array FieldData) := do
---   let goal ← mkFreshMVarId -- no
---   let e ← getEnv
---   let d ← e.find? nm
--- --   guard (isStructureLike e nm)
---   let e_str ← mkAppN (mkConst nm) args
---   let (lctx, cls) ← AddToContext lctx pref e_str
---   IO.println s!"local context: {lctx.decls.toArray}"
---   let sg ← cases goal cls
---   IO.println s!"after cases: {sg.map λ x => x.ctorName}"
---   return (lctx, #[])
--- --   let ctors ← cases goal cls
--- --   let fieldExprs := (ctors.map $ λ x => x.fields).get! 0
--- --   let fields := fieldExprs.map Expr.fvarId!
--- --   let axiom_fields ← fieldExprs.mapM isProof
--- --   let types ← fieldExprs.mapM inferType
--- --   let depends := types.map λ tp => tp.ListFvarIds
--- --   return (fieldExprs.zipWith4 FieldData.mk types depends axiom_fields)
+namespace Meta
+def ppFieldData (x : FieldData) : MetaM Format :=
+do return group (nest 1 (fmt "⟨"  ++
+fmt (← ppExpr x.fvar) ++ fmt "," ++ line ++
+fmt (← ppExpr x.type) ++ fmt "," ++ line ++
+fmt (← x.depends.toList.mapM λ e => ppExpr (mkFVar e)) ++ fmt "," ++ line ++
+fmt x.isProp ++ fmt "⟩"))
 
--- /-- Add fields to context, and returns data -/
--- def AddFieldsToContext (nm : Name) (pref : Name) (args : Array Expr) :
---   TacticM (Array FieldData) := do
---   let e ← getEnv
---   let d ← e.find? nm
--- --   guard (isStructureLike e nm)
---   let e_str ← mkAppN (mkConst nm) args
---   let (lctx, cls) ← AddToContext lctx pref e_str
---   IO.println s!"local context: {lctx.decls.toArray}"
---   let sg ← cases (← getMainGoal) cls
---   IO.println s!"after cases: {sg.map λ x => x.ctorName}"
---   return (lctx, #[])
---   let ctors ← cases goal cls
---   let fieldExprs := (ctors.map $ λ x => x.fields).get! 0
---   let fields := fieldExprs.map Expr.fvarId!
---   let axiom_fields ← fieldExprs.mapM isProof
---   let types ← fieldExprs.mapM inferType
---   let depends := types.map λ tp => tp.ListFvarIds
---   return (fieldExprs.zipWith4 FieldData.mk types depends axiom_fields)
+def AddFieldsToContext (mvarId : MVarId) (nm hnm : Name) (us : List Level) (args : Array Expr) :
+  MetaM (MVarId × Array FieldData) := do
+  let e ← getEnv
+  let d ← e.find? nm
+  let tt ← isStructureLike e nm
+  let eStr ← mkAppN (mkConst nm us) args
+  let (h, mvarId, m2) ← assertm mvarId hnm eStr
+  let l ← cases mvarId h
+  let info := l.get! 0
+  let mvarId := info.mvarId
+  withMVarContext mvarId do
+  let fieldExprs := info.fields
+  let fields := fieldExprs.map Expr.fvarId!
+  let axiom_fields ← fieldExprs.mapM isProof
+  let types ← fieldExprs.mapM inferType
+  let depends := types.map λ tp => tp.ListFvarIds
+  let fieldData := fieldExprs.zipWith4 FieldData.mk types depends axiom_fields
+  IO.println f!"field data: {← fieldData.mapM ppFieldData}"
+  return (mvarId, fieldData)
 
 -- for testing
 def trivialMapping (lctx : LocalContext) (fields1 fields2 : Array FieldData) :
   MetaM $ Array Expr × Array Expr := do
-  let data_fields := fields1.filter $ λ info => !info.isProp
-  let map1 ← data_fields.map λ info => info.fvar
-  let map2 ← data_fields.map λ info => lctx.get! (info.fvar.fvarId!.updateSuffix $ λ s => "h2" ++ s) |>.toExpr
+  let dataFields := fields1.filter $ λ info => !info.isProp
+  let map1 ← dataFields.map λ info => info.fvar
+  let map2 ← dataFields.map λ info => lctx.get! (info.fvar.fvarId!.updateSuffix $ λ s => "h2" ++ s) |>.toExpr
   return (map1, map2)
 
 -- todo
 def allMappings (fields1 fields2 : Array FieldData) : MetaM $ List $ List (FVarId × Expr) := do
- let data_fields1 := fields1.filter $ λ info => !info.isProp
- let data_fields2 := fields2.filter $ λ info => !info.isProp
+ let dataFields1 := fields1.filter $ λ info => !info.isProp
+ let dataFields2 := fields2.filter $ λ info => !info.isProp
  throwError "todo"
 
 
@@ -100,7 +87,7 @@ def matchingAxioms (fields1 fields2 : Array FieldData) (map1 map2 : Array Expr) 
   return same
 
 /-- The tactic we use to automatically prove axioms. -/
-def current_automation : MetaM Unit :=
+def currentAutomation : MetaM Unit :=
 return () -- tidy >> (done <|> tactic.interactive.finish [] none)
 
 -- /-- Tries to prove `e` in the local context, returns tt if successful. -/
@@ -111,109 +98,33 @@ return () -- tidy >> (done <|> tactic.interactive.finish [] none)
 
 /-- Tests whether nm1 is a subclass of nm1. Currently the data fields must have the same Name for
 this tactic to work. -/
--- def is_subclass (nm1 nm2 : Name) (show_state := false) : MetaM Unit := do
---   let lctx := LocalContext.mkEmpty ()
---   let (lctx, M) ← AddToContext lctx `M (mkSort $ mkLevelSucc $ mkLevelParam `u)
---   let (lctx, info1) ← AddFieldsToContext lctx nm1 `h1 #[mkFVar M]
---   let (lctx, info2) ← AddFieldsToContext lctx nm2 `h2 #[mkFVar M]
---   --IO.println s!"{lctx.decls.toList}"
---   let (map1, map2) ← trivialMapping lctx info1 info2
---   let n ← matchingAxioms info1 info2 map1 map2
---   let n_uniqs := n.map λ info => info.fvar.fvarId!
---   let todo := info1.filter λ info => info.isProp && !n_uniqs.contains info.fvar.fvarId!
---   if todo.isEmpty then
---   IO.println s!"{nm1} is a trivial subclass of {nm2}: {nm2} has all the fields that {nm1} has." else do
---   -- trace $ todo.map $ λ info => info.fvar.local_pp_name,
---   -- let cannot_prove ← todo.filterM λ info => bnot <$> try_to_prove (info.type.instantiate_locals mapping),
---   let cannotProve := todo
---   -- trace $ cannot_prove.map $ λ info => info.fvar.local_pp_name,
---   if cannotProve.isEmpty then
---   IO.println s!"{nm1} is a subclass of {nm2}: {nm2} has all the data fields of {nm1}, and all the axioms of {nm1} can be proven from the axioms of {nm2}."
---   else
---   IO.println s!"Cannot prove the following axioms of {nm1} from the axioms of {nm2}:
---   {cannotProve.map $ λ info => info.fvar.fvarId!}."
-
--- run_cmd retrieve $ do
---   e ← get_env,
---   M ← AddToContext `M (Expr.sort $ (level.param `u).succ),
---   let nm := `comm_monoid1,
---   info1 ← AddFieldsToContext `comm_monoid1 `h1 [M],
---   info2 ← AddFieldsToContext `comm_monoid2 `h2 [M],
---   map ← trivialMapping info1 info2,
---   n ← matchingAxioms info1 info2 map,
---   trace n.length,
---   trace map,
---   -- d ← get_decl nm,
---   -- guard $ e.is_structure nm,
---   -- (args, _) ← open_pis d.type,
---   -- e_str ← mk_app nm args,
---   -- cls ← AddToContext `h e_str,
---   -- let args := args ++ [cls],
---   -- field_info ← get_FieldData nm args,
---   -- guard $ field_info.all $ λ info => info.isProp || info.depends.empty, -- no dependent data fields
---   -- data_locals ← field_info.mapM $ λ info => cond info.isProp (return none) $
---   --   (λ x, some (info.field_name, x)) <$> AddToContext info.field_name.last info.type, -- use assertv?
---   -- let data_replacements : name_map Expr :=
---   --   rb_map.of_List data_locals.reduce_option,
---   -- let reduced_types := field_info.filter_map $ λ info => cond info.isProp
---   --   (some $ (info.field_name, info.type.replace_const data_replacements args)) none,
---   -- reduced_types.mapM (λ x, type_check x.2), -- sanity check
---   -- axiom_locals ← reduced_types.mapM $ λ e, AddToContext e.1.last e.2,
---   -- trace reduced_types,
---   -- -- trace $ types,
---   -- trace_state,
---   -- trace field_info,
---   -- trace data_locals,
---   -- trace axiom_locals,
---   -- cases cls,
---   -- trace_state,
---   -- trace $ types.map Expr.to_string,
---   -- trace depends,
---   skip
-
-/-! We define two notions of commutative monoids, the first is right-unital and the second is both left-unital and right-unital. -/
-
-class comm_monoid1 (M : Type _) :=
-(mul : M → M → M)
-(mul_assoc : ∀ x y z, mul (mul x y) z = mul x (mul y z))
-(mul_comm : ∀ x y, mul x y = mul y x)
-(one : M)
-(mul_one : ∀ x, mul x one = x)
-
-#eval (do
-  let env ← getEnv
-  let f := getStructureFields env `comm_monoid1
-  IO.println s!"{f}" : MetaM Unit)
-#print mkMVar
-#print mkFreshExprSyntheticOpaqueMVar
-#print Meta.assert
-
-/--
-  Convert the given goal `Ctx |- target` into `Ctx, name : type |- target` and `Ctx |- type`.
-  It assumes `val` has type `type`.
-  Similar to `assert`, but uses a metavariable for `val`. -/
-def assertm (mvarId : MVarId) (name : Name) (type : Expr) : MetaM (FVarId × MVarId × MVarId) :=
+def isSubclass (mvarId : MVarId) (nm1 nm2 : Name) (show_state := false) : MetaM MVarId := do
+  let u := mkLevelParam `u
+  let (M, mvarId) ← asserti mvarId `M (mkSort (mkLevelSucc u)) (mkConst `PUnit [mkLevelSucc u])
+  let (mvarId, info1) ← AddFieldsToContext mvarId nm1 `h1 [u] #[mkFVar M]
+  let (mvarId, info2) ← AddFieldsToContext mvarId nm2 `h2 [u] #[mkFVar M]
   withMVarContext mvarId do
-    checkNotAssigned mvarId `assert
-    let tag    ← getMVarTag mvarId
-    let target ← getMVarType mvarId
-    let newType := mkForall name BinderInfo.default type target
-    let newMVarFn ← mkFreshExprSyntheticOpaqueMVar newType tag
-    let newMVarB ← mkFreshExprSyntheticOpaqueMVar type tag
-    assignExprMVar mvarId (mkApp newMVarFn newMVarB)
-    let (newFVarId, newMVarId) ← intro1P newMVarFn.mvarId!
-    pure (newFVarId, newMVarId, newMVarB.mvarId!)
+  let (map1, map2) ← trivialMapping (← getLCtx) info1 info2
+  IO.println f!"map 1: {← map1.mapM Meta.ppExpr}"
+  IO.println f!"map 2: {← map2.mapM Meta.ppExpr}"
+  let n ← matchingAxioms info1 info2 map1 map2
+  let n_uniqs := n.map λ info => info.fvar.fvarId!
+  let todo := info1.filter λ info => info.isProp && !n_uniqs.contains info.fvar.fvarId!
+  (if todo.isEmpty then
+  IO.println s!"{nm1} is a trivial subclass of {nm2}: {nm2} has all the fields that {nm1} has." else do
+  -- trace $ todo.map $ λ info => info.fvar.local_pp_name,
+  -- let cannot_prove ← todo.filterM λ info => bnot <$> try_to_prove (info.type.instantiate_locals mapping),
+  let cannotProve := todo
+  -- trace $ cannot_prove.map $ λ info => info.fvar.local_pp_name,
+  if cannotProve.isEmpty then
+  IO.println s!"{nm1} is a subclass of {nm2}: {nm2} has all the data fields of {nm1}, and all the axioms of {nm1} can be proven from the axioms of {nm2}."
+  else
+  IO.println s!"Cannot prove the following axioms of {nm1} from the axioms of {nm2}:
+  {cannotProve.map $ λ info => info.fvar.fvarId!}.")
+  return mvarId
 
-  /--
-Convert the given goal `Ctx |- target` into `Ctx, name : type |- target`.
-It assumes `val` has type `type` -/
-def asserti (mvarId : MVarId) (name : Name) (type : Expr) (val : Expr) : MetaM (FVarId × MVarId) :=
-do
-let m ← assert mvarId name type val
-intro1P m
-
-instance : Inhabited CasesSubgoal :=
-⟨arbitrary, Name.anonymous⟩
+end Meta
+open Meta
 
 def strucTacticM (mvarId : MVarId) : MetaM (MVarId × MVarId × Array FieldData) := do
   let nm := `comm_monoid1
@@ -228,17 +139,13 @@ def strucTacticM (mvarId : MVarId) : MetaM (MVarId × MVarId × Array FieldData)
   let info := l.get! 0
   let mvarId := info.mvarId
   withMVarContext mvarId do
-  IO.println s!"ctorName: {info.ctorName}"
-  IO.println s!"fields: {(← info.fields.mapM λ e => LocalDecl.userName <$> getLocalDecl e.fvarId!)}"
-  IO.println s!"mvarId: {info.mvarId}"
   let fieldExprs := info.fields
   let fields := fieldExprs.map Expr.fvarId!
   let axiom_fields ← fieldExprs.mapM isProof
   let types ← fieldExprs.mapM inferType
   let depends := types.map λ tp => tp.ListFvarIds
   let fieldData := fieldExprs.zipWith4 FieldData.mk types depends axiom_fields
-  IO.println f!"field data: {fieldData}"
-  -- return (fieldExprs.zipWith4 FieldData.mk types depends axiom_fields)
+  IO.println f!"field data: {← fieldData.mapM ppFieldData}"
   return (mvarId, m2, fieldData)
 
 
@@ -271,13 +178,24 @@ syntax (name := struc) "struc" : tactic
     setGoals (m1::m2::l)
   | _ => throwUnsupportedSyntax
 
--- set_option pp.all true
-def foo : Unit := by
-  struc
-  exact ()
+syntax (name := isSubclass) "isSubclass " ident ident : tactic
+@[tactic «isSubclass»] def evalIsSubclass : Tactic := fun stx => do
+  match stx with
+  | `(tactic| isSubclass $nm1 $nm2) => withMainContext do
+    let mvarId ← getMainGoal
+    let mvarId ← Meta.isSubclass mvarId nm1.getId nm2.getId
+    let l ← getUnsolvedGoals
+    setGoals (mvarId::l)
+  | _ => throwUnsupportedSyntax
 
+/-! We define two notions of commutative monoids, the first is right-unital and the second is both left-unital and right-unital. -/
 
-
+class comm_monoid1 (M : Type _) :=
+(mul : M → M → M)
+(mul_assoc : ∀ x y z, mul (mul x y) z = mul x (mul y z))
+(mul_comm : ∀ x y, mul x y = mul y x)
+(one : M)
+(mul_one : ∀ x, mul x one = x)
 
 class comm_monoid2 (M : Type _) :=
 (mul : M → M → M)
@@ -286,6 +204,14 @@ class comm_monoid2 (M : Type _) :=
 (one : M)
 (mul_one : ∀ x, mul x one = x)
 (one_mul : ∀ x, mul one x = x)
+
+example : Unit := by
+  struc
+  exact ()
+
+example : Unit := by
+  isSubclass comm_monoid1 comm_monoid2
+  exact ()
 
 -- #eval is_subclass `comm_monoid1 `comm_monoid2
 /- Output: comm_monoid1 is a trivial subclass of comm_monoid2: comm_monoid2 has all the fields that comm_monoid1 has. -/
